C model for cells

pulse/examples/steel/LListWithTail.Cell.fst
@@ -1,13 +1,49 @@
 module LListWithTail.Cell
 
+(* A Steel model of C cell structs *)
+
 #push-options "--__no_positivity"
 noeq
-type cell (a: Type0) = {
-  next: ref (option (cell a));
-  data: a;
+type mcell (a: Type0) = {
+  data: (data: ref a { ~ (is_null data) });
+  next: (next: ref (option (mcell a)) { ~ (is_null next) });
 }
 #pop-options
 
+let ccell_ptrvalue a = option (mcell a)
+
+let ccell_ptrvalue_null a = None
+
+let ccell_ptrvalue_is_null #a x = None? x
+
+let ccell_data #a c =
+  (Some?.v c).data
+
+let ccell_next #a c =
+  (Some?.v c).next
+
+#push-options "--ide_id_info_off"
+
+let alloc_cell
+  #a data next
+=
+  let rdata = alloc data in
+  change_slprop (pts_to rdata full_perm data `star` emp) (pts_to rdata full_perm data `star` pure (rdata =!= null)) (fun m ->
+    pts_to_not_null rdata full_perm data m;
+    pure_star_interp (pts_to rdata full_perm data) (rdata =!= null) m
+  );
+  elim_pure (rdata =!= null);
+  let rnext = alloc next in
+  change_slprop (pts_to rnext full_perm next `star` emp) (pts_to rnext full_perm next `star` pure (rnext =!= null)) (fun m ->
+    pts_to_not_null rnext full_perm next m;
+    pure_star_interp (pts_to rnext full_perm next) (rnext =!= null) m
+  );
+  elim_pure (rnext =!= null);  
+  let pres = Some ({ data = rdata; next = rnext }) in
+  let gres = Ghost.hide ({ vcell_data = data; vcell_next = next }) in
+  let res = (pres, gres) in
+  change_slprop (pts_to rdata full_perm data `star` pts_to rnext full_perm next) (ccell (fst res) full_perm (snd res)) (fun _ -> ());
+  res
 
 let next c = c.next
 let data c = c.data
