pulse/examples/steel/LListWithTail.Cell.fsti
@@ -1,22 +1,95 @@
 module LListWithTail.Cell
 open Steel.Memory
 open Steel.Effect
+open Steel.Effect.Atomic
 open Steel.FractionalPermission
 open Steel.Reference
 
-val cell (a:Type0) : Type0
-let cellptr (a: Type0) : Type0 = ref (option (cell a))
-val next (c:cell 'a) : cellptr 'a
-val data (c:cell 'a) : 'a
-val mk_cell (n: cellptr 'a) (d:'a)
-  : Pure (cell 'a)
-    (requires True)
-    (ensures fun c ->
-      next c == n /\
-      data c == d)
+(* A C lvalue view of a cell struct, as a pair of two references for its data and next fields *)
+
+val ccell_ptrvalue (a: Type0) : Tot Type0 (* "ccell *" seen as a rvalue, or "ccell * const" *)
+
+val ccell_ptrvalue_null (a: Type0) : Tot (ccell_ptrvalue a)
+
+(* Pointer arithmetic: comparison to null, and pointer to fields. TODO: split these operations between Ghost and Steel, with a proper model of a "permission to do pointer arithmetic without actually reading the value/dereferencing" *)
+
+val ccell_ptrvalue_is_null (#a: Type0) (c: ccell_ptrvalue a) : Pure bool
+  (requires True)
+  (ensures (fun b -> b == true <==> c == ccell_ptrvalue_null a))
+
+let ccell_lvalue (a: Type0) = (c: ccell_ptrvalue a { ccell_ptrvalue_is_null c == false }) (* "ccell" seen as a lvalue. IMPORTANT: one MUST NOT use "ref ccell_lvalue" in C code. In other words, ref can be used to model pointers to rvalues only. *)
+
+val ccell_data (#a: Type0) (c: ccell_lvalue a) : Pure (ref a)
+  (requires True)
+  (ensures (fun v -> ~ (is_null v)))
+
+val ccell_next (#a: Type0) (c: ccell_lvalue a) : Pure (ref (ccell_ptrvalue a))
+  (requires True)
+  (ensures (fun v -> ~ (is_null v)))
+
+(* Important: we DO NOT provide a pure constructor for this data type, since its fields MUST be allocated at the same time and a cell MUST NOT be forged from references that would not come from such same-time allocation. *)
+
+(* The high-level value of a cell (should NEVER be used in C code, only in specs) *)
+
+noeq
+type vcell (a: Type0) = {
+  vcell_data : a;
+  vcell_next : ccell_ptrvalue a;
+}
+
+let ccell (#a: Type0) (c: ccell_lvalue a) (p: perm) (v: Ghost.erased (vcell a)) : Tot slprop =
+  pts_to (ccell_data c) p v.vcell_data `star` pts_to (ccell_next c) p v.vcell_next
+
+let ccellp (#a: Type0) (c: ccell_ptrvalue a) (p: perm) (v: Ghost.erased (option (vcell a))) : Tot slprop =
+  match ccell_ptrvalue_is_null c, Ghost.reveal v with
+  | false, Some v ->
+    let c : ccell_lvalue a = c in
+    ccell c p (Ghost.hide v)
+  | true, None -> emp
+  | _ -> pure False
+
+let ccellp_null_intro (#a: Type0) (c: ccell_ptrvalue a) (p: perm) : Steel unit
+  emp
+  (fun _ -> ccellp c p None)
+  (requires (fun _ -> ccell_ptrvalue_is_null c == true))
+  (ensures (fun _ _ _ -> True))
+= 
+  change_slprop emp (ccellp c p None) (fun _ -> ())
+
+let ccellp_is_null
+  (#a: Type0) (c: ccell_ptrvalue a) (p: perm) (v: Ghost.erased (option (vcell a)))
+: Steel unit
+    (ccellp c p v)
+    (fun _ -> ccellp c p v)
+    (requires (fun _ -> True))
+    (ensures (fun _ _ _ -> ccell_ptrvalue_is_null c == None? (Ghost.reveal v)))
+=
+  change_slprop
+    (ccellp c p v)
+    (ccellp c p v `star` pure (ccell_ptrvalue_is_null c == None? (Ghost.reveal v)))
+    (fun m ->
+      pure_star_interp (ccellp c p v) (ccell_ptrvalue_is_null c == None? (Ghost.reveal v)) m;
+      emp_unit (ccellp c p v);
+      match ccell_ptrvalue_is_null c, Ghost.reveal v with
+      | false, Some _
+      | true, None
+        -> ()
+      | _ -> pure_interp False m
+    );
+  elim_pure (ccell_ptrvalue_is_null c == None? (Ghost.reveal v))
+
+val alloc_cell
+  (#a: Type0)
+  (data: a)
+  (next: ccell_ptrvalue a)
+: Steel (ccell_lvalue a & Ghost.erased (vcell a))
+    emp
+    (fun res -> ccell (fst res) full_perm (snd res))
+    (requires (fun _ -> True))
+    (ensures (fun _ res _ -> Ghost.reveal (snd res) == ({ vcell_data = data; vcell_next = next; })))
 
 let datas
   (#a: Type0)
-  (l: list (cell a))
+  (l: list (vcell a))
 : Tot (list a)
-= List.Tot.map data l
+= List.Tot.map Mkvcell?.vcell_data l
