pulse/examples/steel/LListWithTail.fst
@@ -9,30 +9,30 @@ module L = FStar.List.Tot
 
 noeq
 type t (a: Type0) = {
-  head: cellptr a;
-  tail: cellptr a;
+  head: ccell_ptrvalue a;
+  tail: ccell_ptrvalue a;
 }
 
 let (==) (#a:_) (x y: a) : prop = x == y
 
-let rec llist_fragment (#a:Type) (ptr: cellptr a)
-                                 (l:Ghost.erased (list (cell a)))
+let rec llist_fragment (#a:Type) (ptr: ccell_ptrvalue a)
+                                 (l:Ghost.erased (list (vcell a)))
     : Tot slprop (decreases (Ghost.reveal l))
     =
     match Ghost.reveal l with
     | [] -> emp
     | hd :: tl ->
-      pts_to ptr full_perm (Some hd) `star`
-      llist_fragment (next hd) tl
+      ccellp ptr full_perm (Some hd) `star`
+      llist_fragment hd.vcell_next tl
 
-let llist_fragment_nil (#a: Type) (ptr: cellptr a) (l: Ghost.erased (list (cell a))) : Lemma
+let llist_fragment_nil (#a: Type) (ptr: ccell_ptrvalue a) (l: Ghost.erased (list (vcell a))) : Lemma
   (requires (Nil? l))
   (ensures (llist_fragment ptr l == emp))
 = ()
 
-let llist_fragment_cons (#a: Type) (ptr: cellptr a) (l: Ghost.erased (list (cell a))) : Lemma
+let llist_fragment_cons (#a: Type) (ptr: ccell_ptrvalue a) (l: Ghost.erased (list (vcell a))) : Lemma
   (requires (Cons? l))
-  (ensures (llist_fragment ptr l == (pts_to ptr full_perm (Some (L.hd l)) `star` llist_fragment (next (L.hd l)) (L.tl l))))
+  (ensures (llist_fragment ptr l == (ccellp ptr full_perm (Some (L.hd l)) `star` llist_fragment (L.hd l).vcell_next (L.tl l))))
 = ()
 
 inline_for_extraction noextract let canon () : FStar.Tactics.Tac unit =
@@ -40,32 +40,32 @@ inline_for_extraction noextract let canon () : FStar.Tactics.Tac unit =
 
 let rec next_last
   (#a: Type)
-  (ptr: cellptr a)
-  (l: Ghost.erased (list (cell a)))
-: Tot (Ghost.erased (cellptr a))
+  (ptr: ccell_ptrvalue a)
+  (l: Ghost.erased (list (vcell a)))
+: Tot (Ghost.erased (ccell_ptrvalue a))
   (decreases (Ghost.reveal l))
 =
   match Ghost.reveal l with
   | [] -> Ghost.hide ptr
-  | a :: q -> next_last (next a) q
+  | a :: q -> next_last a.vcell_next q
 
 let rec next_last_correct
   (#a: Type)
-  (ptr: cellptr a)
-  (l: Ghost.erased (list (cell a)))
+  (ptr: ccell_ptrvalue a)
+  (l: Ghost.erased (list (vcell a)))
 : Lemma
   (requires (Cons? l))
-  (ensures (next_last ptr l == Ghost.hide (next (L.last l))))
+  (ensures (next_last ptr l == Ghost.hide (L.last l).vcell_next))
   (decreases (Ghost.reveal l))
 = match Ghost.reveal l with
   | [_] -> ()
-  | a :: q -> next_last_correct (next a) (Ghost.hide q)
+  | a :: q -> next_last_correct a.vcell_next (Ghost.hide q)
 
 let rec llist_fragment_append
   (#a: Type)
-  (ptr: cellptr a)
-  (l1: Ghost.erased (list (cell a)))
-  (l2: Ghost.erased (list (cell a)))
+  (ptr: ccell_ptrvalue a)
+  (l1: Ghost.erased (list (vcell a)))
+  (l2: Ghost.erased (list (vcell a)))
 : Lemma
   (requires True)
   (ensures (((llist_fragment ptr l1 `star` llist_fragment (next_last ptr l1) l2)) `equiv` llist_fragment ptr (l1 `L.append` l2)))
@@ -77,15 +77,15 @@ let rec llist_fragment_append
     ) by canon ()
   | hd :: tl ->
     assert (
-      ((pts_to ptr full_perm (Some hd) `star` llist_fragment (next hd) tl) `star` llist_fragment (next_last (next hd) tl) l2) `equiv`
-      (pts_to ptr full_perm (Some hd) `star` (llist_fragment (next hd) tl `star` llist_fragment (next_last (next hd) tl) l2))
+      ((ccellp ptr full_perm (Some hd) `star` llist_fragment hd.vcell_next tl) `star` llist_fragment (next_last hd.vcell_next tl) l2) `equiv`
+      (ccellp ptr full_perm (Some hd) `star` (llist_fragment hd.vcell_next tl `star` llist_fragment (next_last hd.vcell_next tl) l2))
     ) by (Steel.Memory.Tactics.canon ());
-    llist_fragment_append (next hd) tl l2;
+    llist_fragment_append hd.vcell_next tl l2;
     star_congruence
-      (pts_to ptr full_perm (Some hd))
-      (llist_fragment (next hd) (tl) `star` llist_fragment (next_last (next hd) tl) l2)
-      (pts_to ptr full_perm (Some hd))
-      (llist_fragment (next hd) (tl `L.append` (l2)))
+      (ccellp ptr full_perm (Some hd))
+      (llist_fragment hd.vcell_next (tl) `star` llist_fragment (next_last hd.vcell_next tl) l2)
+      (ccellp ptr full_perm (Some hd))
+      (llist_fragment hd.vcell_next (tl `L.append` (l2)))
 
 (* I wish I had this:
 
@@ -136,51 +136,51 @@ let unsnoc_hd (#a: Type) (l: list a) : Pure (list a) (requires (Cons? l)) (ensur
 let unsnoc_tl (#a: Type) (l: list a) : Pure (a) (requires (Cons? l)) (ensures (fun _ -> True)) = snd (unsnoc l)
 
 [@@__reduce__]
-let llist_with_tail (#a: Type) (x: t a) (l: Ghost.erased (list (cell a))) : Tot slprop =
-  llist_fragment x.head l `star` pts_to (next_last x.head l) full_perm None `star` pure (x.tail == Ghost.reveal (next_last x.head l))
+let llist_with_tail (#a: Type) (x: t a) (l: Ghost.erased (list (vcell a))) : Tot slprop =
+  llist_fragment x.head l `star` ccellp (next_last x.head l) full_perm None `star` pure (x.tail == Ghost.reveal (next_last x.head l))
 
 let create_llist_with_tail (a: Type) : SteelT (t a) emp (fun x -> llist_with_tail x []) =
-  let head : cellptr a = alloc None in
+  let head : ccell_ptrvalue a = ccell_ptrvalue_null a in
   let x : t a = ({ head = head; tail = head; }) in
-//  change_slprop (pts_to head _ _) (pts_to (next_last x.head []) full_perm None) (fun _ -> ());
+  ccellp_null_intro head full_perm;
   intro_pure (x.tail == Ghost.reveal (next_last x.head (Ghost.hide [])));
-  change_slprop (emp `star` pts_to head full_perm None `star` pure (x.tail == Ghost.reveal (next_last x.head (Ghost.hide [])))) (llist_with_tail x []) (fun _ -> ());
+  change_slprop (emp `star` ccellp head full_perm None `star` pure (x.tail == Ghost.reveal (next_last x.head (Ghost.hide [])))) (llist_with_tail x []) (fun _ -> ());
   x
 
 (* BEGIN helpers to unfold definitions just to prove that I can read the head pointer of a list and check its value to determine whether the list is empty or not *)
 
 [@"opaque_to_smt"]
 let read_head_nil
-  (#a: Type) (x: t a) (l: Ghost.erased (list (cell a)))
+  (#a: Type) (x: t a) (l: Ghost.erased (list (vcell a)))
 : Ghost slprop
   (requires (Nil? l))
-  (ensures (fun q -> llist_with_tail x l `equiv` (pts_to x.head full_perm None `star` q)))
+  (ensures (fun q -> llist_with_tail x l `equiv` (ccellp x.head full_perm None `star` q)))
 = assert (
-    (llist_fragment x.head l `star` pts_to (next_last x.head l) full_perm None `star` pure (x.tail == Ghost.reveal (next_last x.head l))) `equiv`
-    (pts_to (next_last x.head l) full_perm None `star` (llist_fragment x.head l `star` pure (x.tail == Ghost.reveal (next_last x.head l))))
+    (llist_fragment x.head l `star` ccellp (next_last x.head l) full_perm None `star` pure (x.tail == Ghost.reveal (next_last x.head l))) `equiv`
+    (ccellp (next_last x.head l) full_perm None `star` (llist_fragment x.head l `star` pure (x.tail == Ghost.reveal (next_last x.head l))))
   ) by canon ();
   (llist_fragment x.head l `star` pure (x.tail == Ghost.reveal (next_last x.head l)))
 
 [@"opaque_to_smt"]
 let read_head_snoc
-  (#a: Type) (x: t a) (l: Ghost.erased (list (cell a)))
+  (#a: Type) (x: t a) (l: Ghost.erased (list (vcell a)))
 : Ghost (slprop)
   (requires (Cons? l))
-  (ensures (fun q -> llist_with_tail x l `equiv` (pts_to x.head full_perm (Some (L.hd l)) `star` q)))
+  (ensures (fun q -> llist_with_tail x l `equiv` (ccellp x.head full_perm (Some (L.hd l)) `star` q)))
 =
   let hd = L.hd l in
   let tl = L.tl l in
   assert (
-    ((pts_to x.head full_perm (Some hd) `star` llist_fragment (next hd) tl) `star` pts_to (next_last x.head l) full_perm None `star` pure (x.tail == Ghost.reveal (next_last x.head l))) `equiv`
-    (pts_to x.head full_perm (Some hd) `star` ((llist_fragment (next hd) tl `star` pts_to (next_last x.head l) full_perm None) `star` pure (x.tail == Ghost.reveal (next_last x.head l))))
+    ((ccellp x.head full_perm (Some hd) `star` llist_fragment hd.vcell_next tl) `star` ccellp (next_last x.head l) full_perm None `star` pure (x.tail == Ghost.reveal (next_last x.head l))) `equiv`
+    (ccellp x.head full_perm (Some hd) `star` ((llist_fragment hd.vcell_next tl `star` ccellp (next_last x.head l) full_perm None) `star` pure (x.tail == Ghost.reveal (next_last x.head l))))
   ) by canon ();
-  (llist_fragment (next hd) tl `star` pts_to (next_last x.head l) full_perm None) `star` pure (x.tail == Ghost.reveal (next_last x.head l))
+  (llist_fragment hd.vcell_next tl `star` ccellp (next_last x.head l) full_perm None) `star` pure (x.tail == Ghost.reveal (next_last x.head l))
 
 let read_head_ghost
-  (#a: Type) (x: t a) (l: Ghost.erased (list (cell a)))
-: Ghost (option (cell a) & slprop)
+  (#a: Type) (x: t a) (l: Ghost.erased (list (vcell a)))
+: Ghost (option (vcell a) & slprop)
   (requires True)
-  (ensures (fun (v, q) -> llist_with_tail x l `equiv` (pts_to x.head full_perm v `star` q) /\ 
+  (ensures (fun (v, q) -> llist_with_tail x l `equiv` (ccellp x.head full_perm v `star` q) /\ 
     v == begin match Ghost.reveal l with 
     | [] -> None
     | a :: _ -> Some a
@@ -209,10 +209,10 @@ let gsnd
 
 [@"opaque_to_smt"]
 let read_head_pure
-  (#a: Type) (x: t a) (l: Ghost.erased (list (cell a)))
-: Pure (Ghost.erased (option (cell a)) & slprop)
+  (#a: Type) (x: t a) (l: Ghost.erased (list (vcell a)))
+: Pure (Ghost.erased (option (vcell a)) & slprop)
   (requires True)
-  (ensures (fun (v, q) -> llist_with_tail x l `equiv` (pts_to x.head full_perm v `star` q) /\ 
+  (ensures (fun (v, q) -> llist_with_tail x l `equiv` (ccellp x.head full_perm v `star` q) /\ 
     Ghost.reveal v == begin match Ghost.reveal l with 
     | [] -> None
     | a :: _ -> Some a
@@ -233,62 +233,78 @@ let change_equiv_slprop
 
 #push-options "--ide_id_info_off"
 
-let read_head
+let is_empty
   (#a: Type)
   (x: t a)
-  (l: Ghost.erased (list (cell a)))
-: Steel (option (cell a))
+  (l: Ghost.erased (list (vcell a)))
+: Steel bool
   (llist_with_tail x l)
   (fun _ -> llist_with_tail x l)
   (requires (fun _ -> True))
   (ensures (fun _ v _ ->
-    v == begin match Ghost.reveal l with 
-    | [] -> None
-    | a :: _ -> Some a
-    end
+    v == Nil? (Ghost.reveal l)
   ))
 =
-  let q : Ghost.erased (option (cell a)) & slprop = read_head_pure x l in
-  change_equiv_slprop (llist_with_tail x l) (pts_to x.head full_perm (fst q) `star` snd q) ();
-  let r = read #(option (cell a)) #full_perm #(fst q) x.head in
-  change_equiv_slprop (pts_to x.head full_perm r `star` snd q)  (llist_with_tail x l) ();
+  let q : Ghost.erased (option (vcell a)) & slprop = read_head_pure x l in
+  change_equiv_slprop (llist_with_tail x l) (ccellp x.head full_perm (fst q) `star` snd q) ();
+  let r = ccell_ptrvalue_is_null x.head in
+  ccellp_is_null x.head full_perm (fst q);
+  change_equiv_slprop (ccellp x.head full_perm (fst q) `star` snd q)  (llist_with_tail x l) ();
   r
 
 (* END helpers to unfold definitions just to prove that I can read the head pointer of a list and check its value to determine whether the list is empty or not *)
 
+noeq
+type dequeue_result (a: Type0) = {
+  dq_val: a;
+  dq_rem: t a;
+  dq_rem_g: Ghost.erased (list (vcell a));
+}
+
 val dequeue
   (#a: Type)
   (x: t a)
-  (l: Ghost.erased (list (cell a)))
-  (next_hd: cellptr a) (* assumed I received this pointer through read_head above *)
-: Steel (t a & Ghost.erased (list (cell a)))
+  (l: Ghost.erased (list (vcell a)))
+: Steel (dequeue_result a)
     (llist_with_tail x l)
-    (fun res -> llist_with_tail (fst res) (snd res))
-    (requires (fun _ -> Cons? l /\ next_hd == next (L.hd l)))
-    (ensures (fun _ res _ -> Cons? l /\ snd res == Ghost.hide (L.tl l) /\ (fst res).tail == x.tail))
+    (fun res -> llist_with_tail (res.dq_rem) (res.dq_rem_g))
+    (requires (fun _ -> Cons? l == true))
+    (ensures (fun _ res _ -> Cons? l /\ res.dq_val == Ghost.reveal (L.hd l).vcell_data /\ res.dq_rem_g == Ghost.hide (L.tl l) /\ res.dq_rem.tail == x.tail))
 
 let dequeue
-  #a x l next_hd
+  #a x l
 =
-  let (l2: Ghost.erased (l: list (cell a) { Cons? l })) = Ghost.hide (Ghost.reveal l) in // necessary otherwise refinement type checking fails
+  let (l2: Ghost.erased (l: list (vcell a) { Cons? l })) = Ghost.hide (Ghost.reveal l) in // necessary otherwise refinement type checking fails
   change_equiv_slprop
     (llist_fragment x.head l)
-    (pts_to x.head full_perm (Some (L.hd l2)) `star` llist_fragment (next (L.hd l2)) (L.tl l2))
+    (ccellp x.head full_perm (Some (L.hd l2)) `star` llist_fragment (L.hd l2).vcell_next (L.tl l2))
     ();
+  ccellp_is_null x.head full_perm (Some (L.hd l2));
+  let hd : ccell_lvalue a = x.head in
+  let pval_hd = ccell_data hd in
+  let pnext_hd = ccell_next hd in
+  change_equiv_slprop
+    (ccellp x.head full_perm (Ghost.hide (Some (L.hd l2))))
+    (pts_to pval_hd full_perm (Ghost.hide (L.hd l2).vcell_data) `star` pts_to pnext_hd full_perm (Ghost.hide (L.hd l2).vcell_next))
+    ();
+  let next_hd = read pnext_hd in
+  let val_hd = read #a #full_perm #(Ghost.hide (L.hd l2).vcell_data) pval_hd in
   let x' = { head = next_hd ; tail = x.tail } in
-  drop (pts_to x.head full_perm (Some (L.hd l2)));
+  let res = { dq_val = val_hd; dq_rem = x' ; dq_rem_g = Ghost.hide (L.tl l2) } in
+  drop (pts_to pval_hd full_perm val_hd);
+  drop (pts_to pnext_hd full_perm next_hd);
   change_slprop
-    (llist_fragment (next (L.hd l2)) (L.tl l2)
-     `star` pts_to (next_last x.head l) full_perm None `star` pure (x.tail == Ghost.reveal (next_last x.head l)))
-    (llist_with_tail x' (L.tl l2))
+    (llist_fragment (L.hd l2).vcell_next (L.tl l2)
+     `star` ccellp (next_last x.head l) full_perm None `star` pure (x.tail == Ghost.reveal (next_last x.head l)))
+    (llist_with_tail res.dq_rem res.dq_rem_g)
     (fun _ -> ());
-  (x', Ghost.hide (L.tl l2))
+  res
 
 let test_read_head_dequeue
   (#a: Type)
   (x: t a)
-  (l: Ghost.erased (list (cell a)))
-: Steel (t a & Ghost.erased (list (cell a)))
+  (l: Ghost.erased (list (vcell a)))
+: Steel (t a & Ghost.erased (list (vcell a)))
     (llist_with_tail x l)
     (fun res -> llist_with_tail (fst res) (snd res))
     (requires (fun _ -> True))
@@ -298,22 +314,23 @@ let test_read_head_dequeue
       | _ :: q -> Ghost.reveal (snd res) == q
     ))
 =
-  let r = read_head x l in
-  match r with
-  | None ->
+  let r = is_empty x l in
+  if r
+  then begin
     noop (); // necessary, otherwise "effects PURE and SteelF cannot be composed"
     (x, l)
-  | Some c ->
-    let n = next c in
-    let res = dequeue x l n in // explicit let-binding necessary, otherwise "effects SteelF and Steel cannot be composed"
-    res
+  end else
+    let res = dequeue x l in
+    (res.dq_rem, res.dq_rem_g)
+
+(* TODO: No longer works because I can no longer overwrite the value pointed to by an "option cell pointer" with a whole cell.
 
 val enqueue
   (#a: Type)
   (x: t a)
-  (l: Ghost.erased (list (cell a)))
+  (l: Ghost.erased (list (vcell a)))
   (v: a)
-: Steel (t a & Ghost.erased (list (cell a)))
+: Steel (t a & Ghost.erased (list (vcell a)))
     (llist_with_tail x l)
     (fun res -> llist_with_tail (fst res) (snd res))
     (requires (fun _ -> True))
@@ -322,8 +339,8 @@ val enqueue
 let enqueue
   #a x l v
 =
-  let n : cellptr a = alloc None in
-  let c = mk_cell n v in
+  let cc = alloc_cell v (ccell_ptrvalue_null a) in
+  let c = Ghost.hide ({ vcell_data = v; vcell_next = ccell_ptrvalue_null a }) in
   elim_pure (x.tail == Ghost.reveal (next_last x.head l));
   change_slprop (pts_to (next_last x.head l) full_perm None) (pts_to x.tail full_perm None) (fun _ -> ());
   write #(option (cell a)) #None x.tail (Some c); // FIXME: WHY WHY WHY do I need to explicitly provide the implicits?
